cnf

cnf.dfy
@@ -21,10 +21,54 @@ module CNF {
     c == f
   }
 
-  // This method simplifies the CNF.
-  method Simp (c : CNF, i : int) returns (n : CNF)
+  function NoDupes (s : set<int>) : bool
+  {
+    
+  }
+  method Abs(i : int) returns (j : int) 
+    ensures j >= 0;
+    ensures i >= 0 ==> i == j && i < 0 ==> j == -i;
+    ensures j >= i;
+    ensures i == j || i == -j;
+  {
+    if i >= 0 {return i;} else {return -i;}
+  }
+
+  // method MaxLitInClause(s : set<int>) returns (j : int) 
+  //   requires s != {}
+  // {
+  //   var ss := s;
+  //   j := 0;
+  //   assert ss == s;
+  //   while ss != {} 
+  //     decreases |ss|
+  //   {
+  //     var i: int :| i in ss;
+  //     var poss := Abs(i);
+  //     assert poss == i || -poss == i;
+  //     assert poss in ss || -poss in ss;
+  //     if poss > j {
+  //       j := poss;
+  //       assert j in ss || -j in ss;
+  //     }
+  //     assert j >= i ;
+  //     ss := ss - {i};
+  //     assert s;
+  //     print(s);
+  //     assert i !in ss;
+  //   }
+  // }
+
+
+  // This method is unit propagation.
+  // It's a little smarter in the sense that
+  // it short circuits when encountering an empty clause.
+  // The responsibility is on the programmer to not have clauses like (1,-1).
+  method UnitProp (c : CNF, i : int) returns (n : CNF)
+    requires forall k :: 0 <= k < c.Length ==> NoDupes(c[k])
     ensures is_true(c) ==> is_true(n)
     ensures is_false(c) ==> is_false(n)
+    ensures |n| <= |c|;
   {
     // c is empty; it is true
     if c == t {return t;}
@@ -33,12 +77,17 @@ module CNF {
     n := [];
     assert |n| == 0;
     assert |n| < |c|;
+
     while k < |c| 
-      invariant 0 <= k <= |c|
+      decreases |c|-k;
+      decreases |c|-|n|;
+      invariant |n| <= k && 0<= k <= |c|;
+      invariant |n| <= |c|;
     {
       if -i in c[k] {
         var elt := c[k] - {-i};
-        // if elt is an empty clause then we derived false.
+        assert |elt| <= |c[k]|;
+        // if elt is an empty clause then we derived false. short circuit
         if elt == {} {return f;}
         assert elt != {};
         n := n + [elt]; 
@@ -50,4 +99,10 @@ module CNF {
     }
     return n;
   }
+}
+
+method Main() {
+  var s := {1, -5, 2};
+  var y := CNF.MaxLitInClause(s);
+  print(s);
 }
